better handle edge case of casting integer to pointer

stdlib/alloc/src/layout.rs
@@ -1,4 +1,5 @@
 #![rr::include("ptr")]
+#![rr::include("result")]
 #![rr::import("stdlib.alloc.theories", "layout")]
 use std::ptr::Alignment;
 
@@ -21,6 +22,9 @@ pub struct Layout {
     align: Alignment,
 }
 
+#[rr::export_as(alloc::alloc::LayoutError)]
+pub struct LayoutError;
+
 #[rr::export_as(alloc::alloc::Layout)]
 impl Layout {
     #[rr::params("x")]
@@ -29,4 +33,46 @@ impl Layout {
     pub const fn size(&self) -> usize {
         self.size
     }
+
+    /*
+    pub const fn from_size_align(size: usize, align: usize) -> Result<Self, LayoutError> {
+        if Layout::is_size_align_valid(size, align) {
+            // SAFETY: Layout::is_size_align_valid checks the preconditions for this call.
+            unsafe { Ok(Layout { size, align: mem::transmute(align) }) }
+        } else {
+            Err(LayoutError)
+        }
+    }
+
+
+
+    const fn is_size_align_valid(size: usize, align: usize) -> bool {
+        let Some(align) = Alignment::new(align) else { return false };
+        if size > Self::max_size_for_align(align) {
+            return false;
+        }
+        true
+    }
+
+    const fn max_size_for_align(align: Alignment) -> usize {
+        // (power-of-two implies align != 0.)
+        // Rounded up size is:
+        //   size_rounded_up = (size + align - 1) & !(align - 1);
+        //
+        // We know from above that align != 0. If adding (align - 1)
+        // does not overflow, then rounding up will be fine.
+        //
+
+        // Conversely, &-masking with !(align - 1) will subtract off
+        // only low-order-bits. Thus if overflow occurs with the sum,
+        // the &-mask cannot subtract enough to undo that overflow.
+        //
+        // Above implies that checking for summation overflow is both
+        // necessary and sufficient.
+
+        // SAFETY: the maximum possible alignment is `isize::MAX + 1`,
+        // so the subtraction cannot overflow.
+        unsafe { unchecked_sub(isize::MAX as usize + 1, align.as_usize()) }
+    }
+    */
 }
