stdlib/mem/src/lib.rs
@@ -1,0 +1,29 @@
+#![feature(register_tool)]
+#![register_tool(rr)]
+#![feature(custom_inner_attributes)]
+
+#![feature(allocator_api)]
+#![rr::package("refinedrust-stdlib")]
+#![rr::coq_prefix("stdlib.mem")]
+#![rr::import("stdlib.mem.theories", "shims")]
+#![allow(unused)]
+
+#[rr::export_as(core::mem::size_of)]
+#[rr::code_shim("mem_size_of")]
+#[rr::returns("ly_size {ly_of T}")]
+pub const fn mem_size_of<T>() -> usize {
+    unimplemented!();
+}
+
+#[rr::export_as(core::mem::align_of)]
+#[rr::code_shim("mem_align_of")]
+#[rr::returns("ly_align {ly_of T}")]
+pub const fn mem_align_of<T>() -> usize {
+    unimplemented!();
+}
+
+#[rr::code_shim("mem_align_log_of")]
+#[rr::returns("ly_align_log {ly_of T}")]
+pub const fn mem_align_log_of<T>() -> usize {
+    unimplemented!();
+}
