stdlib/mem/output/mem/proofs/proof_mem_align_of.v
@@ -1,11 +1,11 @@
 From caesium Require Import lang notation.
 From refinedrust Require Import typing shims.
-From stdlib.ptr.ptr.generated Require Import generated_code_ptr generated_specs_ptr generated_template_mem_align_of.
+From stdlib.mem.mem.generated Require Import generated_code_mem generated_specs_mem generated_template_mem_align_of.
 
 Set Default Proof Using "Type".
 
 Section proof.
-Context `{RRGS : !refinedrustGS Σ}.
+Context `{!refinedrustGS Σ}.
 
 Lemma mem_align_of_proof (π : thread_id) :
   mem_align_of_lemma π.
