stdlib/mem/output/mem/proofs/proof_mem_size_of.v
@@ -1,23 +1,22 @@
 From caesium Require Import lang notation.
 From refinedrust Require Import typing shims.
-From stdlib.ptr.ptr.generated Require Import generated_code_ptr generated_specs_ptr generated_template_mem_align_log_of.
+From stdlib.mem.mem.generated Require Import generated_code_mem generated_specs_mem generated_template_mem_size_of.
 
 Set Default Proof Using "Type".
 
 Section proof.
-Context `{RRGS : !refinedrustGS Σ}.
+Context `{!refinedrustGS Σ}.
 
-Lemma mem_align_log_of_proof (π : thread_id) :
-  mem_align_log_of_lemma π.
+Lemma mem_size_of_proof (π : thread_id) :
+  mem_size_of_lemma π.
 Proof.
-  mem_align_log_of_prelude.
+  mem_size_of_prelude.
 
   repeat liRStep; liShow.
 
   all: print_remaining_goal.
   Unshelve. all: sidecond_solver.
   Unshelve. all: sidecond_hammer.
-  by apply ly_align_log_in_usize.
   Unshelve. all: print_remaining_sidecond.
 Qed.
 End proof.
