stdlib/mem/theories/shims.v
@@ -1,0 +1,39 @@
+From caesium Require Import lang notation.
+From refinedrust Require Import annotations.
+
+
+Definition mem_size_of `{!LayoutAlg} (T_st : syn_type) : function := {|
+  f_args := [];
+  f_local_vars := [("ret", USize : layout); ("_1", use_layout_alg' UnitSynType); ("_2", use_layout_alg' UnitSynType)];
+  f_code :=
+    <["_bb0" :=
+      "ret" <-{IntOp USize} (i2v (ly_size (use_layout_alg' T_st)) USize);
+      return (use{IntOp USize} "ret")
+    ]>%E $
+    ∅;
+  f_init := "_bb0";
+|}.
+
+Definition mem_align_of `{!LayoutAlg} (T_st : syn_type) : function := {|
+  f_args := [];
+  f_local_vars := [("ret", USize : layout); ("_1", use_layout_alg' UnitSynType); ("_2", use_layout_alg' UnitSynType)];
+  f_code :=
+    <["_bb0" :=
+    "ret" <-{IntOp USize} (i2v (ly_align (use_layout_alg' T_st)) USize);
+    return (use{IntOp USize} "ret")
+    ]>%E $
+    ∅;
+  f_init := "_bb0";
+|}.
+
+Definition mem_align_log_of `{!LayoutAlg} (T_st : syn_type) : function := {|
+  f_args := [];
+  f_local_vars := [("ret", USize : layout); ("_1", use_layout_alg' UnitSynType); ("_2", use_layout_alg' UnitSynType)];
+  f_code :=
+    <["_bb0" :=
+    "ret" <-{IntOp USize} (i2v (ly_align_log (use_layout_alg' T_st)) USize);
+    return (use{IntOp USize} "ret")
+    ]>%E $
+    ∅;
+  f_init := "_bb0";
+|}.
