stdlib/rr_internal/theories/shims.v
@@ -107,7 +107,8 @@ Proof.
   { rewrite /has_layout_loc/layout_wf/aligned_to /ly_align/=. destruct caesium_config.enforce_alignment; last done. apply Z.divide_1_l. }
   { rewrite /has_layout_loc/layout_wf/aligned_to /ly_align/=. destruct caesium_config.enforce_alignment; last done. apply Z.divide_1_l. }
   { rewrite /has_layout_val length_drop/=. rewrite Hlen/new_ly/ly_size/=.  lia.  }
-  { rewrite ly_align_mk_array_layout.
+  { rewrite /ly_align_in_bounds.
+    rewrite ly_align_mk_array_layout.
     unsafe_unfold_common_caesium_defs.
     sidecond_hammer. }
 Qed.
